# 1

$$
\lim_{ x \to 0 } \sqrt[x]{ 1-3x } = \lim_{ x \to 0 } (1-3x)^{\frac{1}{2}} = (1^{\infty}) = \lim_{ x \to 0 } (1-3x)^{\frac{1}{-3x} \frac{-3x}{x}} = e^{-3}
$$

# 2

$$
\lim_{ x \to \frac{\pi}{2} } \left( \frac{1+\cos{x}}{1+ cotan{x}} \right)^{\frac{1}{x-\frac{\pi}{2}}} = \lim_{ x \to \frac{\pi}{2} } \left( \frac{1+\cos{x}}{1+ \frac{\cos{x}}{\sin{x}}} \right)^{\frac{1}{x-\frac{\pi}{2}}} = \lim_{ x \to \frac{\pi}{2} } \left( \frac{1+\cos{x}}{\frac{\sin{x}+\cos{x}}{\sin{x}}} \right)^{\frac{1}{x-\frac{\pi}{2}}} = \lim_{ x \to \frac{\pi}{2} } \left( \frac{(1+\cos{x})\sin{x}}{\sin{x}+\cos{x}} \right)^{\frac{1}{x-\frac{\pi}{2}}}
$$

$$
x-\frac{\pi}{2} = t \quad x=t+\frac{\pi}{2}
$$

$$
\lim_{ t \to 0 } \left( \frac{\left(1+\cos\left( \frac{\pi}{2} +t \right)\right)}{1+ cotan\left(  \frac{\pi}{2} + t  \right)} \right) = \dots = \lim_{ t \to 0 } (1+\frac{\tan{t}-\sin{t}}{1-\tan{t}})^{\frac{1}{t}}
$$

$$
\lim_{ x \to \frac{\pi}{2} } \left( \frac{1+\cos{x}}{1+cotan{x}} \right)^{\frac{1}{x-\frac{\pi}{2}}} = \dots = \lim_{ x \to \frac{\pi}{2} } \left( 1 + \frac{-cotan{x} + \cos{x}}{1 + cotan{x}} \right)^{\frac{1}{x-\frac{\pi}{2}}} = e^{\lim_{ x \to \frac{\pi}{2} } \frac{-cotan{x} + \cos{x}}{(1+cotan{x})\left( x-\frac{\pi}{2} \right)} } = e^{\lim_{ t \to 0 } } \frac{\left( -cotan\left( \frac{\pi}{2} + t \right) + \cos\left( \frac{\pi}{2} + t \right) \right)}{1 + cotan\left( \frac{\pi}{2 + t} \right)t} = \dots = e^1
$$

# 3

$$
\alpha(x) = \sin{\sqrt{x \sqrt{ x } }} \quad \beta{x} = \sqrt{ x^2 + \sqrt{ x^3 } } \quad x_{0} = 0
$$

$$
\lim_{ x \to 0 } \frac{\sin {\sqrt{ x \sqrt{ x } }}}{\sqrt{ x^2 \sqrt{ x^3 } }}
$$
